common/Memdata.v
@@ -118,6 +118,8 @@ Qed.
   content of a memory cell.  It can be either:
 - a concrete 8-bit integer;
 - a byte-sized fragment of an opaque pointer;
+- a special construct [PointerPad] that represents the padding belonging
+  to a single pointer fragment written as an integer.
 - the special constant [Undef] that represents uninitialized memory.
 *)
 
@@ -126,7 +128,8 @@ Qed.
 Inductive memval: Type :=
   | Undef: memval
   | Byte: byte -> memval
-  | Pointer: block -> int -> nat -> memval.
+  | Pointer: block -> int -> nat -> memval
+  | PointerPad : memval.
 
 (** * Encoding and decoding integers *)
 
@@ -145,15 +148,6 @@ Fixpoint int_of_bytes (l: list byte): Z :=
   | b :: l' => Byte.unsigned b + int_of_bytes l' * 256
   end.
 
-Definition rev_if_be (l: list byte) : list byte :=
-  if Archi.big_endian then List.rev l else l.
-
-Definition encode_int (sz: nat) (x: Z) : list byte :=
-  rev_if_be (bytes_of_int sz x).
-
-Definition decode_int (b: list byte) : Z :=
-  int_of_bytes (rev_if_be b).
-
 (** Length properties *)
 
 Lemma length_bytes_of_int:
@@ -162,18 +156,10 @@ Proof.
   induction n; simpl; intros. auto. decEq. auto.
 Qed.
 
-Lemma rev_if_be_length:
-  forall l, length (rev_if_be l) = length l.
+Lemma bytes_of_int_length:
+  forall sz x, length (bytes_of_int sz x) = sz.
 Proof.
-  intros; unfold rev_if_be; destruct Archi.big_endian.
-  apply List.rev_length.
-  auto.
-Qed.
-
-Lemma encode_int_length:
-  forall sz x, length(encode_int sz x) = sz.
-Proof.
-  intros. unfold encode_int. rewrite rev_if_be_length. apply length_bytes_of_int.
+  intros. apply length_bytes_of_int.
 Qed.
 
 (** Decoding after encoding *)
@@ -184,7 +170,6 @@ Lemma int_of_bytes_of_int:
 Proof.
   induction n; intros.
   simpl. rewrite Zmod_1_r. auto.
-Opaque Byte.wordsize.
   rewrite inj_S. simpl.
   replace (Zsucc (Z_of_nat n) * 8) with (Z_of_nat n * 8 + 8) by omega.
   rewrite two_p_is_exp; try omega. 
@@ -194,49 +179,80 @@ Opaque Byte.wordsize.
   apply two_p_gt_ZERO. omega. apply two_p_gt_ZERO. omega.
 Qed.
 
-Lemma rev_if_be_involutive:
-  forall l, rev_if_be (rev_if_be l) = l.
+Lemma int_of_bytes_of_int_1:
+  forall x, Int.repr (int_of_bytes (bytes_of_int 1 (Int.unsigned x))) = Int.zero_ext 8 x.
 Proof.
-  intros; unfold rev_if_be; destruct Archi.big_endian. 
-  apply List.rev_involutive. 
-  auto.
-Qed.
-
-Lemma decode_encode_int:
-  forall n x, decode_int (encode_int n x) = x mod (two_p (Z_of_nat n * 8)).
-Proof.
-  unfold decode_int, encode_int; intros. rewrite rev_if_be_involutive. 
-  apply int_of_bytes_of_int.
-Qed.
-
-Lemma decode_encode_int_1:
-  forall x, Int.repr (decode_int (encode_int 1 (Int.unsigned x))) = Int.zero_ext 8 x.
-Proof.
-  intros. rewrite decode_encode_int. 
+  intros. rewrite int_of_bytes_of_int. 
   rewrite <- (Int.repr_unsigned (Int.zero_ext 8 x)).
   decEq. symmetry. apply Int.zero_ext_mod. compute. intuition congruence. 
 Qed.
 
-Lemma decode_encode_int_2:
-  forall x, Int.repr (decode_int (encode_int 2 (Int.unsigned x))) = Int.zero_ext 16 x.
+Lemma int_of_bytes_of_int_2:
+  forall x, Int.repr (int_of_bytes (bytes_of_int 2 (Int.unsigned x))) = Int.zero_ext 16 x.
 Proof.
-  intros. rewrite decode_encode_int. 
+  intros. rewrite int_of_bytes_of_int. 
   rewrite <- (Int.repr_unsigned (Int.zero_ext 16 x)).
-  decEq. symmetry. apply Int.zero_ext_mod. compute; intuition congruence.
+  decEq. symmetry. apply Int.zero_ext_mod. compute. intuition congruence. 
 Qed.
 
-Lemma decode_encode_int_4:
-  forall x, Int.repr (decode_int (encode_int 4 (Int.unsigned x))) = x.
+Lemma int_of_bytes_of_int_4:
+  forall x, Int.repr (int_of_bytes (bytes_of_int 4 (Int.unsigned x))) = x.
 Proof.
-  intros. rewrite decode_encode_int. transitivity (Int.repr (Int.unsigned x)).
+  intros. rewrite int_of_bytes_of_int. transitivity (Int.repr (Int.unsigned x)).
   decEq. apply Zmod_small. apply Int.unsigned_range. apply Int.repr_unsigned.
 Qed.
 
-Lemma decode_encode_int_8:
-  forall x, Int64.repr (decode_int (encode_int 8 (Int64.unsigned x))) = x.
+Lemma int_of_bytes_of_int_8:
+  forall x, Int64.repr (int_of_bytes (bytes_of_int 8 (Int64.unsigned x))) = x.
 Proof.
-  intros. rewrite decode_encode_int. transitivity (Int64.repr (Int64.unsigned x)).
+  intros. rewrite int_of_bytes_of_int. transitivity (Int64.repr (Int64.unsigned x)).
   decEq. apply Zmod_small. apply Int64.unsigned_range. apply Int64.repr_unsigned.
+Qed.
+
+Lemma int_of_bytes_append:
+  forall l2 l1, 
+  int_of_bytes (l1 ++ l2) = int_of_bytes l1 + int_of_bytes l2 * two_p (Z_of_nat (length l1) * 8).
+Proof.
+  induction l1; simpl int_of_bytes; intros.
+  simpl. ring.
+  simpl length. rewrite inj_S. 
+  replace (Z.succ (Z.of_nat (length l1)) * 8) with (Z_of_nat (length l1) * 8 + 8) by omega.
+  rewrite two_p_is_exp. change (two_p 8) with 256. rewrite IHl1. ring.
+  omega. omega.
+Qed.
+
+Lemma int_of_bytes_range:
+  forall l, 0 <= int_of_bytes l < two_p (Z_of_nat (length l) * 8).
+Proof.
+  induction l; intros. 
+  simpl. omega.
+  simpl length. rewrite inj_S. 
+  replace (Z.succ (Z.of_nat (length l)) * 8) with (Z.of_nat (length l) * 8 + 8) by omega.
+  rewrite two_p_is_exp. change (two_p 8) with 256. 
+  simpl int_of_bytes. generalize (Byte.unsigned_range a). 
+  change Byte.modulus with 256. omega. 
+  omega. omega. 
+Qed.
+
+Lemma bytes_of_int_append:
+  forall n2 x2 n1 x1,
+  0 <= x1 < two_p (Z_of_nat n1 * 8) ->
+  bytes_of_int (n1 + n2) (x1 + x2 * two_p (Z_of_nat n1 * 8)) =
+  bytes_of_int n1 x1 ++ bytes_of_int n2 x2.
+Proof.
+  induction n1; intros.
+- simpl in *. f_equal. omega. 
+- assert (E: two_p (Z.of_nat (S n1) * 8) = two_p (Z.of_nat n1 * 8) * 256).
+  {
+    rewrite inj_S. change 256 with (two_p 8). rewrite <- two_p_is_exp. 
+    f_equal. omega. omega. omega. 
+  }
+  rewrite E in *. simpl. f_equal.
+  apply Byte.eqm_samerepr. exists (x2 * two_p (Z.of_nat n1 * 8)). 
+  change Byte.modulus with 256. ring.
+  rewrite Zmult_assoc. rewrite Z_div_plus. apply IHn1.
+  apply Zdiv_interval_1. omega. apply two_p_gt_ZERO; omega. omega. 
+  assumption. omega.
 Qed.
 
 (** A length-[n] encoding depends only on the low [8*n] bits of the integer. *)
@@ -261,21 +277,17 @@ Proof.
   rewrite <- Z_div_plus_full_l. decEq. change (two_p 8) with 256. ring. omega.
 Qed.
 
-Lemma encode_int_8_mod:
+Lemma bytes_of_int_8_mod:
   forall x y,
   Int.eqmod (two_p 8) x y ->
-  encode_int 1%nat x = encode_int 1%nat y.
-Proof.
-  intros. unfold encode_int. decEq. apply bytes_of_int_mod. auto.
-Qed.
+  bytes_of_int 1 x = bytes_of_int 1 y.
+Proof. apply (bytes_of_int_mod 1). Qed.
 
-Lemma encode_int_16_mod:
+Lemma bytes_of_int_16_mod:
   forall x y,
   Int.eqmod (two_p 16) x y ->
-  encode_int 2%nat x = encode_int 2%nat y.
-Proof.
-  intros. unfold encode_int. decEq. apply bytes_of_int_mod. auto.
-Qed.
+  bytes_of_int 2 x = bytes_of_int 2 y.
+Proof. apply (bytes_of_int_mod 2). Qed.
 
 (** * Encoding and decoding values *)
 
@@ -317,6 +329,12 @@ Fixpoint inj_pointer (n: nat) (b: block) (ofs: int) {struct n}: list memval :=
   | S m => Pointer b ofs m :: inj_pointer m b ofs
   end.
 
+Definition inj_pointer_seg (n : nat) (b: block) (ofs: int) (i : nat) : list memval :=
+  match n with
+  | O => nil
+  | S m => Pointer b ofs i :: list_repeat m PointerPad
+  end.
+
 Fixpoint check_pointer (n: nat) (b: block) (ofs: int) (vl: list memval) 
                        {struct n} : bool :=
   match n, vl with
@@ -326,53 +344,25 @@ Fixpoint check_pointer (n: nat) (b: block) (ofs: int) (vl: list memval)
   | _, _ => false
   end.
 
-Definition proj_pointer (vl: list memval) : val :=
+Definition proj_pointer (vl: list memval) : option (block * int) :=
   match vl with
   | Pointer b ofs n :: vl' =>
-      if check_pointer 4%nat b ofs vl then Vptr b ofs else Vundef
-  | _ => Vundef
+     if check_pointer 4 b ofs vl then Some (b, ofs) else None
+  | _ => None
   end.
 
-Definition encode_val (chunk: memory_chunk) (v: val) : list memval :=
-  match v, chunk with
-  | Vint n, (Mint8signed | Mint8unsigned) => inj_bytes (encode_int 1%nat (Int.unsigned n))
-  | Vint n, (Mint16signed | Mint16unsigned) => inj_bytes (encode_int 2%nat (Int.unsigned n))
-  | Vint n, Mint32 => inj_bytes (encode_int 4%nat (Int.unsigned n))
-  | Vptr b ofs, Mint32 => inj_pointer 4%nat b ofs
-  | Vlong n, Mint64 => inj_bytes (encode_int 8%nat (Int64.unsigned n))
-  | Vfloat n, Mfloat32 => inj_bytes (encode_int 4%nat (Int.unsigned (Float.bits_of_single n)))
-  | Vfloat n, Mfloat64 => inj_bytes (encode_int 8%nat (Int64.unsigned (Float.bits_of_double n)))
-  | _, _ => list_repeat (size_chunk_nat chunk) Undef
+Fixpoint check_pointer_pad (n: nat) (vl: list memval) : bool :=
+  match n, vl with
+  | O, nil => true
+  | S m, PointerPad :: vl' => check_pointer_pad m vl'
+  | _, _ => false
   end.
-
-Definition decode_val (chunk: memory_chunk) (vl: list memval) : val :=
-  match proj_bytes vl with
-  | Some bl =>
-      match chunk with
-      | Mint8signed => Vint(Int.sign_ext 8 (Int.repr (decode_int bl)))
-      | Mint8unsigned => Vint(Int.zero_ext 8 (Int.repr (decode_int bl)))
-      | Mint16signed => Vint(Int.sign_ext 16 (Int.repr (decode_int bl)))
-      | Mint16unsigned => Vint(Int.zero_ext 16 (Int.repr (decode_int bl)))
-      | Mint32 => Vint(Int.repr(decode_int bl))
-      | Mint64 => Vlong(Int64.repr(decode_int bl))
-      | Mfloat32 => Vfloat(Float.single_of_bits (Int.repr (decode_int bl)))
-      | Mfloat64 => Vfloat(Float.double_of_bits (Int64.repr (decode_int bl)))
-      end
-  | None =>
-      match chunk with
-      | Mint32 => proj_pointer vl
-      | _ => Vundef
-      end
+Definition proj_pointer_seg (n : nat) (vl: list memval) : option (block * int * nat) :=
+  match n, vl with
+  | S m, Pointer b ofs i :: vl' =>
+     if check_pointer_pad m vl' then Some (b, ofs, i) else None
+  | _, _ => None
   end.
-
-Lemma encode_val_length:
-  forall chunk v, length(encode_val chunk v) = size_chunk_nat chunk.
-Proof.
-  intros. destruct v; simpl; destruct chunk; 
-  solve [ reflexivity
-        | apply length_list_repeat
-        | rewrite length_inj_bytes; apply encode_int_length ].
-Qed.
 
 Lemma check_inj_pointer:
   forall b ofs n, check_pointer n b ofs (inj_pointer n b ofs) = true.
@@ -381,6 +371,206 @@ Proof.
   unfold proj_sumbool. rewrite dec_eq_true. rewrite dec_eq_true.  
   rewrite <- beq_nat_refl. simpl; auto.
 Qed.
+Lemma check_repeat_pointer_pad:
+  forall n, check_pointer_pad n (list_repeat n PointerPad) = true.
+Proof.
+  induction n; simpl; auto. 
+Qed.
+
+Lemma proj_inj_pointer:
+  forall b ofs, proj_pointer (inj_pointer 4 b ofs) = Some (b, ofs).
+Proof.
+  intros. change (proj_pointer (inj_pointer 4 b ofs)) with
+    (if check_pointer 4 b ofs (inj_pointer 4 b ofs) then Some (b, ofs) else None).
+  now rewrite check_inj_pointer.
+Qed.
+
+Lemma proj_inj_pointer_seg:
+  forall n b ofs i,
+  (0 < n)%nat ->
+  proj_pointer_seg n (inj_pointer_seg n b ofs i) = Some (b, ofs, i).
+Proof.
+  intros. destruct n as [|n]; [omega|].
+  unfold inj_pointer_seg. unfold proj_pointer_seg.
+  now rewrite check_repeat_pointer_pad.
+Qed.
+
+Lemma proj_inj_pointer_seg_None:
+  forall n b ofs i, proj_pointer (inj_pointer_seg n b ofs i) = None.
+Proof.
+  intros. destruct n as [|[|?]]; simpl; rewrite ?andb_false_r; auto.
+Qed.
+
+Lemma check_pointer_inv:
+  forall b ofs n mv,
+  check_pointer n b ofs mv = true -> mv = inj_pointer n b ofs.
+Proof.
+  induction n; destruct mv; simpl; auto; try discriminate.
+  destruct m; try discriminate. intro.
+  rewrite !andb_true_iff in H. destruct H as [[[??]?]?].
+  apply beq_nat_true in H1. apply proj_sumbool_true in H.
+  apply proj_sumbool_true in H0. subst. now rewrite (IHn mv).
+Qed.
+
+Lemma proj_pointer_inv:
+  forall b ofs mv,
+  proj_pointer mv = Some (b,ofs) -> mv = inj_pointer 4 b ofs.
+Proof.
+  intros. apply (check_pointer_inv b ofs 4 mv).
+  destruct mv as [|[]]; try discriminate. unfold proj_pointer in *.
+  destruct (check_pointer _ b0 _ _) eqn:?; congruence.
+Qed.
+
+Lemma check_pointer_pad_inv:
+  forall n mv,
+  check_pointer_pad n mv = true -> mv = list_repeat n PointerPad.
+Proof.
+  induction n; destruct mv; simpl; auto; try discriminate.
+  destruct m; try discriminate. intros; f_equal; auto.
+Qed.
+
+Lemma proj_pointer_seg_inv:
+  forall n b ofs i mv,
+  proj_pointer_seg n mv = Some (b,ofs,i) -> mv = inj_pointer_seg n b ofs i.
+Proof.
+  intros [|n] b ofs i [|[]] ?; simpl in *; try discriminate.
+  destruct (check_pointer_pad _ _) eqn:?; inv H.
+  now erewrite <-check_pointer_pad_inv by eauto.
+Qed.
+
+Lemma length_proj_bytes:
+  forall l b, proj_bytes l = Some b -> length b = length l.
+Proof.
+  induction l; simpl; intros. 
+  inv H; auto.
+  destruct a; try discriminate. 
+  destruct (proj_bytes l) eqn:E; inv H. 
+  simpl. f_equal. auto.
+Qed.
+
+Lemma proj_bytes_append:
+  forall l2 l1,
+  proj_bytes (l1 ++ l2) =
+  match proj_bytes l1, proj_bytes l2 with
+  | Some b1, Some b2 => Some (b1 ++ b2)
+  | _, _ => None
+  end.
+Proof.
+  induction l1; simpl.
+  destruct (proj_bytes l2); auto.
+  destruct a; auto. rewrite IHl1. 
+  destruct (proj_bytes l1); auto. destruct (proj_bytes l2); auto. 
+Qed.
+
+Arguments bytes_of_int _ _ : simpl never.
+Arguments int_of_bytes _ : simpl never.
+Arguments proj_bytes _ : simpl never.
+Arguments inj_bytes _ : simpl never.
+Arguments check_pointer _ _ _ _ : simpl never.
+Arguments check_pointer_pad _ _ : simpl never.
+Arguments inj_pointer _ _ _ : simpl never.
+Arguments inj_pointer_seg _ _ _ _ : simpl never.
+Arguments proj_pointer _ : simpl never.
+Arguments proj_pointer_seg _ _ : simpl never.
+
+
+Definition rev_if_be {A} (l: list A) : list A :=
+  if Archi.big_endian then List.rev_append l nil else l.
+
+Lemma rev_if_be_length:
+  forall (A: Type) (l : list A), length (rev_if_be l) = length l.
+Proof.
+  intros. unfold rev_if_be. destruct Archi.big_endian; auto.
+  now rewrite rev_append_rev, app_nil_r, List.rev_length.
+Qed.
+Lemma rev_if_be_involutive:
+  forall (A: Type) (l : list A), rev_if_be (rev_if_be l) = l.
+Proof.
+  intros. unfold rev_if_be. destruct Archi.big_endian; auto.
+  now rewrite !rev_append_rev, !app_nil_r, List.rev_involutive. 
+Qed.
+Lemma rev_if_be_repeat:
+  forall (A : Type) n (x : A), rev_if_be (list_repeat n x) = list_repeat n x.
+Proof.
+  intros. unfold rev_if_be. destruct Archi.big_endian; auto.
+  rewrite rev_append_rev, app_nil_r.
+  induction n; intros; simpl; auto.
+  change (x :: nil) with (list_repeat 1 x).
+  now rewrite IHn, <-list_repeat_plus, plus_comm.
+Qed.
+Lemma in_rev_if_be:
+  forall (A : Type) (x : A) (l : list A), In x (rev_if_be l) <-> In x l.
+Proof.
+  intros. unfold rev_if_be. now destruct Archi.big_endian;
+    rewrite ?rev_append_rev, ?app_nil_r, <-?in_rev.
+Qed.
+Lemma rev_if_be_forall2:
+  forall (A B : Type) (P : A -> B -> Prop) l1 l2,
+  list_forall2 P l1 l2 -> list_forall2 P (rev_if_be l1) (rev_if_be l2).
+Proof.
+  intros until 0. unfold rev_if_be. destruct Archi.big_endian; auto.
+  rewrite !rev_append_rev, !app_nil_r.
+  induction 1; simpl.
+  * constructor.
+  * apply list_forall2_app; repeat constructor; auto.
+Qed.
+Lemma rev_if_be_app:
+  forall (A : Type) (l1 l2 : list A), rev_if_be (l1 ++ l2) =
+    rev_if_be (if Archi.big_endian then l2 else l1) ++
+    rev_if_be (if Archi.big_endian then l1 else l2).
+Proof.
+  intros. unfold rev_if_be. destruct Archi.big_endian; auto.
+  now rewrite !rev_append_rev, !app_nil_r, rev_app_distr.
+Qed.
+
+Definition encode_val (chunk: memory_chunk) (v: val) : list memval :=
+  rev_if_be
+  match v, chunk with
+  | Vint n, (Mint8signed | Mint8unsigned) => inj_bytes (bytes_of_int 1 (Int.unsigned n))
+  | Vint n, (Mint16signed | Mint16unsigned) => inj_bytes (bytes_of_int 2 (Int.unsigned n))
+  | Vint n, Mint32 => inj_bytes (bytes_of_int 4 (Int.unsigned n))
+  | Vptrseg b ofs i, (Mint8signed | Mint8unsigned) => inj_pointer_seg 1 b ofs i
+  | Vptrseg b ofs i, Mint32 => inj_pointer_seg 4 b ofs i
+  | Vptr b ofs, Mint32 => inj_pointer 4 b ofs
+  | Vlong n, Mint64 => inj_bytes (bytes_of_int 8 (Int64.unsigned n))
+  | Vfloat n, Mfloat32 => inj_bytes (bytes_of_int 4 (Int.unsigned (Float.bits_of_single n)))
+  | Vfloat n, Mfloat64 => inj_bytes (bytes_of_int 8 (Int64.unsigned (Float.bits_of_double n)))
+  | _, _ => list_repeat (size_chunk_nat chunk) Undef
+  end.
+
+Definition decode_val (chunk: memory_chunk) (vl: list memval) : val :=
+  let vl := rev_if_be vl in
+  match proj_bytes vl with
+  | Some bl =>
+      match chunk with
+      | Mint8signed => Vint (Int.sign_ext 8 (Int.repr (int_of_bytes bl)))
+      | Mint8unsigned => Vint (Int.zero_ext 8 (Int.repr (int_of_bytes bl)))
+      | Mint16signed => Vint (Int.sign_ext 16 (Int.repr (int_of_bytes bl)))
+      | Mint16unsigned => Vint (Int.zero_ext 16 (Int.repr (int_of_bytes bl)))
+      | Mint32 => Vint (Int.repr (int_of_bytes bl))
+      | Mint64 => Vlong (Int64.repr (int_of_bytes bl))
+      | Mfloat32 => Vfloat (Float.single_of_bits (Int.repr (int_of_bytes bl)))
+      | Mfloat64 => Vfloat(Float.double_of_bits (Int64.repr (int_of_bytes bl)))
+      end
+  | None =>
+      match chunk with
+      | Mint32 =>
+          match proj_pointer vl with
+          | Some (b,ofs) => Vptr b ofs
+          | None =>
+              match proj_pointer_seg 4 vl with
+              | Some (b,ofs,i) => Vptrseg b ofs i
+              | None => Vundef
+              end
+          end
+      | Mint8signed | Mint8unsigned =>
+          match proj_pointer_seg 1 vl with
+          | Some (b,ofs,i) => Vptrseg b ofs i
+          | None => Vundef
+          end
+      | _ => Vundef
+      end
+  end.
 
 Definition decode_encode_val (v1: val) (chunk1 chunk2: memory_chunk) (v2: val) : Prop :=
   match v1, chunk1, chunk2 with
@@ -403,6 +593,9 @@ Definition decode_encode_val (v1: val) (chunk1 chunk2: memory_chunk) (v2: val) :
   | Vlong n, Mint64, Mfloat64 => v2 = Vfloat(Float.double_of_bits n)
   | Vlong n, (Mint8signed|Mint8unsigned|Mint16signed|Mint16unsigned|Mint32|Mfloat32|Mfloat64), _ => v2 = Vundef
   | Vlong n, _, _ => True (**r nothing meaningful to say about v2 *)
+  | Vptrseg b ofs i, (Mint8signed | Mint8unsigned), (Mint8signed | Mint8unsigned) => v2 = Vptrseg b ofs i
+  | Vptrseg b ofs i, Mint32, Mint32 => v2 = Vptrseg b ofs i
+  | Vptrseg b ofs i, _, _ => v2 = Vundef
   | Vfloat f, Mfloat32, Mfloat32 => v2 = Vfloat(Float.singleoffloat f)
   | Vfloat f, Mfloat32, Mint32 => v2 = Vint(Float.bits_of_single f)
   | Vfloat f, Mfloat64, Mfloat64 => v2 = Vfloat f
@@ -411,40 +604,36 @@ Definition decode_encode_val (v1: val) (chunk1 chunk2: memory_chunk) (v2: val) :
   | Vfloat f, _, _ => True   (* nothing interesting to say about v2 *)
   end.
 
-Remark decode_val_undef:
-  forall bl chunk, decode_val chunk (Undef :: bl) = Vundef.
+Lemma encode_val_length:
+  forall chunk v, length (encode_val chunk v) = size_chunk_nat chunk.
 Proof.
-  intros. unfold decode_val. simpl. destruct chunk; auto.
+  intros. unfold encode_val. rewrite rev_if_be_length.
+  now destruct v, chunk; rewrite ?length_list_repeat,
+    ?length_inj_bytes, ?length_bytes_of_int.
+Qed.
+
+Lemma decode_val_repeat_undef:
+  forall chunk n, (0 < n)%nat -> decode_val chunk (list_repeat n Undef) = Vundef.
+Proof.
+  intros. unfold decode_val. rewrite rev_if_be_repeat.
+  destruct n. omega. destruct chunk; reflexivity.
 Qed.
 
 Lemma decode_encode_val_general:
   forall v chunk1 chunk2,
   decode_encode_val v chunk1 chunk2 (decode_val chunk2 (encode_val chunk1 v)).
 Proof.
-Opaque inj_pointer.
-  intros.
-  destruct v; destruct chunk1; simpl; try (apply decode_val_undef);
-  destruct chunk2; unfold decode_val; auto; try (rewrite proj_inj_bytes).
-  rewrite decode_encode_int_1. decEq. apply Int.sign_ext_zero_ext. omega.
-  rewrite decode_encode_int_1. decEq. apply Int.zero_ext_idem. omega.
-  rewrite decode_encode_int_1. decEq. apply Int.sign_ext_zero_ext. omega.
-  rewrite decode_encode_int_1. decEq. apply Int.zero_ext_idem. omega.
-  rewrite decode_encode_int_2. decEq. apply Int.sign_ext_zero_ext. omega.
-  rewrite decode_encode_int_2. decEq. apply Int.zero_ext_idem. omega.
-  rewrite decode_encode_int_2. decEq. apply Int.sign_ext_zero_ext. omega.
-  rewrite decode_encode_int_2. decEq. apply Int.zero_ext_idem. omega.
-  rewrite decode_encode_int_4. auto.
-  rewrite decode_encode_int_4. auto.
-  rewrite decode_encode_int_8. auto.
-  rewrite decode_encode_int_8. auto.
-  rewrite decode_encode_int_4. auto.
-  rewrite decode_encode_int_4. decEq. apply Float.single_of_bits_of_single.
-  rewrite decode_encode_int_8. auto.
-  rewrite decode_encode_int_8. decEq. apply Float.double_of_bits_of_double.
-  change (proj_bytes (inj_pointer 4 b i)) with (@None (list byte)). simpl. 
-  unfold proj_pointer. generalize (check_inj_pointer b i 4%nat).
-Transparent inj_pointer. 
-  simpl. intros EQ; rewrite EQ; auto.
+  intros. unfold decode_val, encode_val. rewrite rev_if_be_involutive.
+  destruct v, chunk1, chunk2; auto;
+    unfold decode_encode_val; rewrite
+    ?proj_inj_bytes, ?int_of_bytes_of_int_1, ?int_of_bytes_of_int_2,
+    ?int_of_bytes_of_int_4, ?int_of_bytes_of_int_8,
+    ?Int.sign_ext_zero_ext, ?Int.zero_ext_idem,
+    ?Float.single_of_bits_of_single, ?Float.double_of_bits_of_double by omega; auto.
+  * now rewrite proj_inj_pointer.
+  * now rewrite proj_inj_pointer_seg_None.
+  * now rewrite proj_inj_pointer_seg_None.
+  * now rewrite proj_inj_pointer_seg_None.
 Qed.
 
 Lemma decode_encode_val_similar:
@@ -463,14 +652,13 @@ Lemma decode_val_type:
   forall chunk cl,
   Val.has_type (decode_val chunk cl) (type_of_chunk chunk).
 Proof.
-  intros. unfold decode_val. 
-  destruct (proj_bytes cl). 
-  destruct chunk; simpl; auto. apply Float.single_of_bits_is_single.
-  destruct chunk; simpl; auto.
-  unfold proj_pointer. destruct cl; try (exact I).
-  destruct m; try (exact I).
-  destruct (check_pointer 4%nat b i (Pointer b i n :: cl));
-  exact I.
+  intros. unfold decode_val.
+  destruct (proj_bytes _), chunk; simpl; auto.
+  * apply Float.single_of_bits_is_single.
+  * destruct (proj_pointer_seg 1 _) as [[[??]?]|]; simpl; auto.
+  * destruct (proj_pointer_seg 1 _) as [[[??]?]|]; simpl; auto.
+  * destruct (proj_pointer _) as [[??]|]; simpl; auto.
+    destruct (proj_pointer_seg 4 _) as [[[??]?]|]; simpl; auto.
 Qed.
 
 Lemma encode_val_int8_signed_unsigned:
@@ -478,60 +666,253 @@ Lemma encode_val_int8_signed_unsigned:
 Proof.
   intros. destruct v; simpl; auto.
 Qed.
-
 Lemma encode_val_int16_signed_unsigned:
   forall v, encode_val Mint16signed v = encode_val Mint16unsigned v.
 Proof.
   intros. destruct v; simpl; auto.
 Qed.
-
 Lemma encode_val_int8_zero_ext:
   forall n, encode_val Mint8unsigned (Vint (Int.zero_ext 8 n)) = encode_val Mint8unsigned (Vint n).
 Proof.
-  intros; unfold encode_val. decEq. apply encode_int_8_mod. apply Int.eqmod_zero_ext. 
-  compute; intuition congruence.
+  intros; unfold encode_val. rewrite (bytes_of_int_mod _ _ (Int.unsigned n)); auto.
+  apply Int.eqmod_zero_ext. compute; intuition congruence.
 Qed.
-
 Lemma encode_val_int8_sign_ext:
   forall n, encode_val Mint8signed (Vint (Int.sign_ext 8 n)) = encode_val Mint8signed (Vint n).
 Proof.
-  intros; unfold encode_val. decEq. apply encode_int_8_mod. apply Int.eqmod_sign_ext'. compute; auto.
+  intros; unfold encode_val. rewrite (bytes_of_int_mod _ _ (Int.unsigned n)); auto.
+  apply Int.eqmod_sign_ext'. compute; intuition congruence.
 Qed.
-
 Lemma encode_val_int16_zero_ext:
   forall n, encode_val Mint16unsigned (Vint (Int.zero_ext 16 n)) = encode_val Mint16unsigned (Vint n).
 Proof.
-  intros; unfold encode_val. decEq. apply encode_int_16_mod. apply Int.eqmod_zero_ext. compute; intuition congruence.
+  intros; unfold encode_val. rewrite (bytes_of_int_mod _ _ (Int.unsigned n)); auto.
+  apply Int.eqmod_zero_ext. compute; intuition congruence.
 Qed.
-
 Lemma encode_val_int16_sign_ext:
   forall n, encode_val Mint16signed (Vint (Int.sign_ext 16 n)) = encode_val Mint16signed (Vint n).
 Proof.
-  intros; unfold encode_val. decEq. apply encode_int_16_mod. apply Int.eqmod_sign_ext'. compute; auto.
+  intros; unfold encode_val. rewrite (bytes_of_int_mod _ _ (Int.unsigned n)); auto.
+  apply Int.eqmod_sign_ext'. compute; intuition congruence.
 Qed.
 
 Lemma decode_val_cast:
   forall chunk l,
   let v := decode_val chunk l in
   match chunk with
-  | Mint8signed => v = Val.sign_ext 8 v
-  | Mint8unsigned => v = Val.zero_ext 8 v
+  | Mint8signed => ~is_ptrseg v -> v = Val.sign_ext 8 v
+  | Mint8unsigned => ~is_ptrseg v -> v = Val.zero_ext 8 v
   | Mint16signed => v = Val.sign_ext 16 v
   | Mint16unsigned => v = Val.zero_ext 16 v
   | Mfloat32 => v = Val.singleoffloat v
   | _ => True
   end.
 Proof.
-  unfold decode_val; intros; destruct chunk; auto; destruct (proj_bytes l); auto.
-  unfold Val.sign_ext. rewrite Int.sign_ext_idem; auto. omega.
-  unfold Val.zero_ext. rewrite Int.zero_ext_idem; auto. omega. 
-  unfold Val.sign_ext. rewrite Int.sign_ext_idem; auto. omega.
-  unfold Val.zero_ext. rewrite Int.zero_ext_idem; auto. omega.
-  simpl. rewrite Float.singleoffloat_of_bits. auto.
+  unfold decode_val; intros; destruct chunk; auto; destruct (proj_bytes _); auto.
+  * unfold Val.sign_ext. rewrite Int.sign_ext_idem; auto. omega.
+  * destruct (proj_pointer_seg _ _) as [[[??]?]|]; simpl; auto. now intros [].
+  * unfold Val.zero_ext. rewrite Int.zero_ext_idem; auto. omega.
+  * destruct (proj_pointer_seg _ _) as [[[??]?]|]; simpl; auto. now intros [].
+  * unfold Val.sign_ext. rewrite Int.sign_ext_idem; auto. omega.
+  * unfold Val.zero_ext. rewrite Int.zero_ext_idem; auto. omega.
+  * simpl. rewrite Float.singleoffloat_of_bits. auto.
+Qed.
+Lemma decode_val_int8_signed_unsigned:
+  forall l,
+  ~is_ptrseg (decode_val Mint8signed l) ->
+  decode_val Mint8signed l = Val.sign_ext 8 (decode_val Mint8unsigned l).
+Proof.
+  intros. rewrite (decode_val_cast Mint8signed) by auto.
+  unfold decode_val. destruct (proj_bytes _); [|reflexivity].
+  simpl. now rewrite Int.sign_ext_zero_ext, Int.sign_ext_idem by omega.
+Qed.
+Lemma decode_val_int8_signed_unsigned_ptrseg:
+  forall l,
+  is_ptrseg (decode_val Mint8signed l) <-> is_ptrseg (decode_val Mint8unsigned l).
+Proof.
+  intros. unfold decode_val. destruct (proj_bytes _).
+  * split; inversion 1.
+  * reflexivity.
+Qed.
+Lemma decode_val_int8_signed_unsigned_alt:
+  forall l,
+  decode_val Mint8signed l = Val.sign_ext_8_alt (decode_val Mint8unsigned l).
+Proof.
+  intros. unfold decode_val. destruct (proj_bytes _).
+  * simpl. now rewrite Int.sign_ext_zero_ext.
+  * now destruct (proj_pointer_seg _ _) as [[[??]?]|].
+Qed.
+
+Lemma decode_val_int16_signed_unsigned:
+  forall l,
+  decode_val Mint16signed l = Val.sign_ext 16 (decode_val Mint16unsigned l).
+Proof.
+  intros. rewrite (decode_val_cast Mint16signed).
+  unfold decode_val. destruct (proj_bytes _); [|reflexivity].
+  simpl. now rewrite Int.sign_ext_zero_ext, Int.sign_ext_idem by omega.
+Qed.
+
+Lemma decode_val_pointer_inv:
+  forall chunk mvl b ofs,
+  decode_val chunk mvl = Vptr b ofs ->
+  chunk = Mint32 /\ mvl = rev_if_be (inj_pointer 4 b ofs).
+Proof.
+  unfold decode_val. intros.
+  destruct (proj_bytes _), chunk; try congruence.
+  * destruct (proj_pointer_seg _ _) as [[[??]?]|]; discriminate.
+  * destruct (proj_pointer_seg _ _) as [[[??]?]|]; discriminate.
+  * destruct (proj_pointer _) as [[??]|] eqn:?.
+    { inv H. now rewrite <-(proj_pointer_inv _ _ (rev_if_be mvl)),
+        rev_if_be_involutive. }
+    destruct (proj_pointer_seg _ _) as [[[??]?]|]; discriminate.
+Qed.
+
+Lemma in_inj_bytes:
+  forall mv bl, In mv (inj_bytes bl) -> exists b, mv = Byte b /\ In b bl.
+Proof.
+  induction bl; simpl; firstorder eauto.
+Qed.
+Lemma in_inj_pointer:
+  forall mv n b ofs, In mv (inj_pointer n b ofs) -> exists i, mv = Pointer b ofs i.
+Proof.
+  induction n; simpl; intuition eauto.
+Qed.
+Lemma in_inj_pointer_seg:
+  forall mv n b ofs i, In mv (inj_pointer_seg n b ofs i) ->
+  mv = Pointer b ofs i \/ (mv = PointerPad /\ n <> 1%nat).
+Proof.
+  intros mv [|n] b ofs i; [intros []|intros [?|?]; auto].
+  right. split. eauto using in_list_repeat. destruct n; intuition.
+Qed.
+
+Local Ltac simplify_in_inj :=
+  repeat match goal with
+    | _ => discriminate
+    | H : In _ (list_repeat _ _) |- _ =>
+      apply in_list_repeat in H; subst
+    | H : In _ (inj_pointer _ _ _) |- _ =>
+      apply in_inj_pointer in H; destruct H; subst
+    | H : In _ (inj_bytes _) |- _ =>
+      apply in_inj_bytes in H; destruct H as (?&?&?); subst
+    | H : In _ (inj_pointer_seg _ _ _ _) |- _ =>
+      apply in_inj_pointer_seg in H; destruct H as [?|[??]]; subst
+    | H : Pointer _ _ _ = Pointer _ _ _ |- _ =>
+      injection H; clear H; intros; subst
+    end.
+
+Lemma inj_pointer_encode_val_overlap:
+  forall chunk n v mv b ofs,
+  In mv (inj_pointer n b ofs) -> In mv (encode_val chunk v) ->
+  chunk <> Mint32 ->
+  exists i, (chunk = Mint8signed \/ chunk = Mint8unsigned) /\ v = Vptrseg b ofs i.
+Proof.
+  intros chunk n v mv b ofs INJ ENC CNK.
+  unfold encode_val in ENC; rewrite in_rev_if_be in ENC.
+  destruct chunk, v; simplify_in_inj; intuition eauto.
+Qed.
+
+Lemma decode_val_pointer_seg_inv:
+  forall chunk mvl b ofs i,
+  decode_val chunk mvl = Vptrseg b ofs i ->
+  (chunk = Mint8signed \/ chunk = Mint8unsigned \/ chunk = Mint32) /\
+  mvl = rev_if_be (inj_pointer_seg (size_chunk_nat chunk) b ofs i).
+Proof.
+  unfold decode_val. intros.
+  destruct (proj_bytes _), chunk; try congruence.
+  * destruct (proj_pointer_seg _ _) as [[[??]?]|] eqn:?; inv H.
+    erewrite <-proj_pointer_seg_inv, rev_if_be_involutive by eauto; auto.
+  * destruct (proj_pointer_seg _ _) as [[[??]?]|] eqn:?; inv H.
+    erewrite <-proj_pointer_seg_inv, rev_if_be_involutive by eauto; auto.
+  * destruct (proj_pointer _) as [[??]|] eqn:?; inv H.
+    destruct (proj_pointer_seg _ _) as [[[??]?]|] eqn:?; inv H1.
+    erewrite <-(proj_pointer_seg_inv 4), rev_if_be_involutive by eauto; auto.
+Qed.
+
+Lemma inj_pointer_seg_encode_val_overlap:
+  forall chunk n v mv b ofs i,
+  In mv (inj_pointer_seg n b ofs i) -> In mv (encode_val chunk v) ->
+  chunk <> Mint32 ->
+  (chunk = Mint8signed \/ chunk = Mint8unsigned) /\ v = Vptrseg b ofs i.
+Proof.
+  intros chunk n v mv b ofs i INJ ENC CNK.
+  unfold encode_val in ENC; rewrite in_rev_if_be in ENC.
+  destruct chunk, v; simplify_in_inj; intuition eauto.
+Qed.
+
+Lemma inj_pointer_seg_1_encode_val_overlap:
+  forall chunk v mv b ofs i,
+  In mv (inj_pointer_seg 1 b ofs i) -> In mv (encode_val chunk v) ->
+  (chunk = Mint32 /\ v = Vptr b ofs)
+  \/ (chunk = Mint8signed \/ chunk = Mint8unsigned \/ chunk = Mint32) /\ v = Vptrseg b ofs i.
+Proof.
+  intros chunk v mv b ofs i INJ ENC.
+  unfold encode_val in ENC; rewrite in_rev_if_be in ENC.
+  destruct chunk, v; simplify_in_inj; intuition eauto.
+Qed.
+
+(** * Breaking 64-bit memory accesses into two 32-bit accesses *)
+Lemma decode_val_int64:
+  forall l1 l2,
+  length l1 = 4%nat -> length l2 = 4%nat ->
+  decode_val Mint64 (l1 ++ l2) =
+  Val.longofwords (decode_val Mint32 (if Archi.big_endian then l1 else l2))
+                  (decode_val Mint32 (if Archi.big_endian then l2 else l1)).
+Proof.
+  intros. unfold decode_val. rewrite !rev_if_be_app, proj_bytes_append.
+  destruct (proj_bytes (rev_if_be (if Archi.big_endian then l2 else l1))) as [b1|] eqn:?,
+    (proj_bytes (rev_if_be (if Archi.big_endian then l1 else l2))) as [b2|] eqn:?;
+    repeat match goal with
+    | |- context [ proj_pointer ?l ] => destruct (proj_pointer l) as [[??]|]
+    | |- context [ proj_pointer_seg ?n ?l ] => destruct (proj_pointer_seg n l) as [[[??]?]|]
+    end; try reflexivity.
+  assert (UR: forall b,
+    length b = 4%nat -> Int.unsigned (Int.repr (int_of_bytes b)) = int_of_bytes b).
+  { intros b Hb. apply Int.unsigned_repr.
+    generalize (int_of_bytes_range b). rewrite Hb.
+    change (two_p (Z.of_nat 4 * 8)) with (Int.max_unsigned + 1). omega. }
+  assert (length b1 = 4%nat) as Hb1.
+  { erewrite length_proj_bytes, rev_if_be_length by eauto. now destruct Archi.big_endian. }
+  assert (length b2 = 4%nat) as Hb2.
+  { erewrite length_proj_bytes, rev_if_be_length by eauto. now destruct Archi.big_endian. }
+  rewrite int_of_bytes_append; simpl. rewrite Int64.ofwords_add, !UR, Hb1 by easy.
+  now rewrite Z.add_comm.
+Qed.
+
+Lemma bytes_of_int64:
+  forall i,
+  bytes_of_int 8 (Int64.unsigned i) =
+  bytes_of_int 4 (Int.unsigned (Int64.loword i)) ++ bytes_of_int 4 (Int.unsigned (Int64.hiword i)).
+Proof.
+  intros. transitivity (bytes_of_int (4 + 4) (Int64.unsigned (Int64.ofwords (Int64.hiword i) (Int64.loword i)))).
+  f_equal. f_equal. rewrite Int64.ofwords_recompose. auto.
+  rewrite Int64.ofwords_add'.
+  change 32 with (Z_of_nat 4 * 8). 
+  rewrite Zplus_comm. apply bytes_of_int_append. apply Int.unsigned_range. 
+Qed.
+
+Lemma encode_val_int64:
+  forall v,
+  encode_val Mint64 v =
+     encode_val Mint32 (if Archi.big_endian then Val.hiword v else Val.loword v)
+  ++ encode_val Mint32 (if Archi.big_endian then Val.loword v else Val.hiword v).
+Proof.
+  intros. destruct v; unfold encode_val, rev_if_be; destruct Archi.big_endian eqn:BI; try reflexivity.
+  * unfold Val.loword, Val.hiword, encode_val, inj_bytes.
+    now rewrite !rev_append_rev, !app_nil_r, <-rev_app_distr, <-map_app, bytes_of_int64.
+  * unfold Val.loword, Val.hiword, encode_val, inj_bytes.
+    now rewrite <-map_app, bytes_of_int64.
 Qed.
 
 (** Pointers cannot be forged. *)
 
+Inductive pointer_bytes_valid (b : block) (ofs : int) :
+    nat -> list memval -> Prop :=
+  | pointer_bytes_valid_nil : pointer_bytes_valid b ofs 0 nil
+  | pointer_bytes_valid_cons n mws :
+     pointer_bytes_valid b ofs n mws ->
+     pointer_bytes_valid b ofs (S n) (Pointer b ofs n :: mws).
+
+(*
 Definition memval_valid_first (mv: memval) : Prop :=
   match mv with
   | Pointer b ofs n => n = 3%nat
@@ -667,6 +1048,7 @@ Proof.
   intros. exploit decode_val_pointer_inv; eauto. intros [A B].
   split; auto. subst mvl. apply encode_pointer_shape. 
 Qed.
+*)
 
 (** * Compatibility with memory injections *)
 
@@ -680,6 +1062,8 @@ Inductive memval_inject (f: meminj): memval -> memval -> Prop :=
       f b1 = Some (b2, delta) ->
       ofs2 = Int.add ofs1 (Int.repr delta) ->
       memval_inject f (Pointer b1 ofs1 n) (Pointer b2 ofs2 n)
+  | memval_inject_ptr_pad:
+      memval_inject f PointerPad PointerPad
   | memval_inject_undef:
       forall mv, memval_inject f Undef mv.
 
@@ -699,11 +1083,24 @@ Lemma proj_bytes_inject:
   proj_bytes vl = Some bl ->
   proj_bytes vl' = Some bl.
 Proof.
-  induction 1; simpl. congruence.
-  inv H; try congruence.
-  destruct (proj_bytes al); intros. 
-  inv H. rewrite (IHlist_forall2 l); auto. 
-  congruence.
+  intros. apply inj_proj_bytes in H0.
+  cut (vl' = inj_bytes bl).
+  { intros. subst. apply proj_inj_bytes. }
+  subst. revert vl' H.
+  induction bl; inversion_clear 1; auto.
+  inv H0. unfold inj_bytes; fold inj_bytes; simpl; decEq; auto.
+Qed.
+Lemma proj_bytes_not_inject:
+  forall f vl vl' bs,
+  list_forall2 (memval_inject f) vl vl' ->
+  proj_bytes vl = None -> proj_bytes vl' = Some bs -> In Undef vl.
+Proof.
+  intros until 1. revert bs.
+  induction H; simpl; unfold proj_bytes; fold proj_bytes; intros; [discriminate |].
+  inv H; try intuition congruence.
+  destruct (proj_bytes al); try discriminate.
+  destruct (proj_bytes bl); try discriminate.
+  eauto.
 Qed.
 
 Lemma check_pointer_inject:
@@ -714,63 +1111,101 @@ Lemma check_pointer_inject:
   f b = Some(b', delta) ->
   check_pointer n b' (Int.add ofs (Int.repr delta)) vl' = true.
 Proof.
-  induction 1; intros; destruct n; simpl in *; auto. 
-  inv H; auto.
-  destruct (andb_prop _ _ H1). destruct (andb_prop _ _ H). 
-  destruct (andb_prop _ _ H5). 
-  assert (n = n0) by (apply beq_nat_true; auto).
-  assert (b = b0) by (eapply proj_sumbool_true; eauto). 
-  assert (ofs = ofs1) by (eapply proj_sumbool_true; eauto).
-  subst. rewrite H3 in H2; inv H2. 
-  unfold proj_sumbool. rewrite dec_eq_true. rewrite dec_eq_true. 
-  rewrite <- beq_nat_refl. simpl. eauto. 
-  congruence.
+  intros. apply check_pointer_inv in H0. subst.
+  cut (vl' = inj_pointer n b' (Int.add ofs (Int.repr delta))).
+  { intros. subst. apply check_inj_pointer. }
+  revert vl' H. induction n; unfold inj_pointer; fold inj_pointer;
+    inversion_clear 1; auto.
+  f_equal. inv H0. congruence. auto.
 Qed.
-
 Lemma proj_pointer_inject:
   forall f vl1 vl2,
   list_forall2 (memval_inject f) vl1 vl2 ->
-  val_inject f (proj_pointer vl1) (proj_pointer vl2).
+  forall b ofs,
+  proj_pointer vl1 = Some (b,ofs) ->
+  exists b' delta,
+  f b = Some (b', delta) /\
+  proj_pointer vl2 = Some (b', Int.add ofs (Int.repr delta)).
 Proof.
-  intros. unfold proj_pointer.
-  inversion H; subst. auto. inversion H0; subst; auto.
-  case_eq (check_pointer 4%nat b0 ofs1 (Pointer b0 ofs1 n :: al)); intros.
-  exploit check_pointer_inject. eexact H. eauto. eauto. 
-  intro. rewrite H4. econstructor; eauto. 
-  constructor.
+  destruct 1; try discriminate.
+  unfold proj_pointer. intros. destruct H; try discriminate.
+  destruct (check_pointer 4 b1 _ _) eqn:?; inv H1.
+  exists b2, delta. erewrite check_pointer_inject; eauto.
+  constructor. econstructor; eauto. auto.
 Qed.
 
-Lemma proj_bytes_not_inject:
+Lemma check_pointer_pad_inject:
   forall f vl vl',
   list_forall2 (memval_inject f) vl vl' ->
-  proj_bytes vl = None -> proj_bytes vl' <> None -> In Undef vl.
+  forall n,
+  check_pointer_pad n vl = true ->
+  check_pointer_pad n vl' = true.
 Proof.
-  induction 1; simpl; intros.
-  congruence.
-  inv H; try congruence. 
-  right. apply IHlist_forall2.
-  destruct (proj_bytes al); congruence.
-  destruct (proj_bytes bl); congruence.
-  auto.
+  induction 1; intros [|?];
+    unfold check_pointer_pad; fold check_pointer_pad; auto.
+  destruct H; try discriminate; auto.
+Qed.
+Lemma proj_pointer_seg_inject:
+  forall f vl1 vl2,
+  list_forall2 (memval_inject f) vl1 vl2 ->
+  forall n b ofs i,
+  proj_pointer_seg n vl1 = Some (b,ofs,i) ->
+  exists b' delta,
+  f b = Some (b', delta) /\
+  proj_pointer_seg n vl2 = Some (b', Int.add ofs (Int.repr delta), i).
+Proof.
+  destruct 1; intros [|?]; try discriminate.
+  unfold proj_pointer_seg. intros. destruct H; try discriminate.
+  destruct (check_pointer_pad n al) eqn:?; inv H1.
+  exists b2, delta. erewrite check_pointer_pad_inject; eauto.
 Qed.
 
 Lemma check_pointer_undef:
   forall n b ofs vl,
   In Undef vl -> check_pointer n b ofs vl = false.
 Proof.
-  induction n; intros; simpl. 
-  destruct vl. elim H. auto.
-  destruct vl. auto.
-  destruct m; auto. simpl in H; destruct H. congruence.
-  rewrite IHn; auto. apply andb_false_r. 
+  induction n; intros ?? [|??]; simpl; intuition auto; subst.
+  * reflexivity.
+  * unfold check_pointer; fold check_pointer.
+    now destruct m; rewrite ?IHn, ?andb_false_r by auto.
 Qed.
-
 Lemma proj_pointer_undef:
-  forall vl, In Undef vl -> proj_pointer vl = Vundef.
+  forall vl, In Undef vl -> proj_pointer vl = None.
 Proof.
   intros; unfold proj_pointer.
-  destruct vl; auto. destruct m; auto. 
-  rewrite check_pointer_undef. auto. auto.
+  destruct vl as [|[]?]; auto. now rewrite check_pointer_undef.
+Qed.
+
+Lemma check_pointer_pad_undef:
+  forall n vl,
+  In Undef vl -> check_pointer_pad n vl = false.
+Proof.
+  induction n; intros [|??]; simpl; intuition auto; subst.
+  * reflexivity.
+  * unfold check_pointer_pad; fold check_pointer_pad.
+    destruct m; auto.
+Qed.
+Lemma proj_pointer_seg_undef:
+  forall n vl, In Undef vl -> proj_pointer_seg n vl = None.
+Proof.
+  intros; unfold proj_pointer_seg.
+  destruct n; auto.
+  destruct vl as [|[]?]; auto.
+  destruct H; try discriminate.
+  now rewrite check_pointer_pad_undef.
+Qed.
+
+Lemma proj_pointer_seg_not_pointer:
+  forall f vl1 vl2,
+  list_forall2 (memval_inject f) vl1 vl2 ->
+  forall b ofs i,
+  proj_pointer_seg 4 vl1 = Some (b, ofs, i) ->
+  proj_pointer vl2 = None.
+Proof.
+  destruct 1; try discriminate. inv H; try discriminate.
+  unfold proj_pointer, proj_pointer_seg. intros.
+  destruct H0; try discriminate. inv H0; try discriminate.
+  unfold check_pointer. simpl. now rewrite !andb_false_r.
 Qed.
 
 Theorem decode_val_inject:
@@ -778,14 +1213,38 @@ Theorem decode_val_inject:
   list_forall2 (memval_inject f) vl1 vl2 ->
   val_inject f (decode_val chunk vl1) (decode_val chunk vl2).
 Proof.
-  intros. unfold decode_val. 
-  case_eq (proj_bytes vl1); intros. 
-  exploit proj_bytes_inject; eauto. intros. rewrite H1. 
-  destruct chunk; constructor.
+  intros. unfold decode_val.
+  destruct (proj_bytes (rev_if_be vl1)) eqn:?.
+  { exploit (proj_bytes_inject f (rev_if_be vl1) (rev_if_be vl2));
+      eauto using rev_if_be_forall2.
+    intros. rewrite H0. destruct chunk; constructor. }
   destruct chunk; auto.
-  case_eq (proj_bytes vl2); intros.
-  rewrite proj_pointer_undef. auto. eapply proj_bytes_not_inject; eauto. congruence.
-  apply proj_pointer_inject; auto.
+  * destruct (proj_bytes (rev_if_be vl2)) eqn:?.
+    { rewrite proj_pointer_seg_undef;
+        eauto using proj_bytes_not_inject, rev_if_be_forall2. }
+    destruct (proj_pointer_seg 1 (rev_if_be vl1)) as [[[??]?]|] eqn:?; [|constructor].
+    exploit (proj_pointer_seg_inject f (rev_if_be vl1) (rev_if_be vl2));
+      eauto using rev_if_be_forall2.
+    intros (?&?&?&E). rewrite E. econstructor; eauto.
+  * destruct (proj_bytes (rev_if_be vl2)) eqn:?.
+    { rewrite proj_pointer_seg_undef;
+        eauto using proj_bytes_not_inject, rev_if_be_forall2. }
+    destruct (proj_pointer_seg 1 (rev_if_be vl1)) as [[[??]?]|] eqn:?; [|constructor].
+    exploit (proj_pointer_seg_inject f (rev_if_be vl1) (rev_if_be vl2));
+      eauto using rev_if_be_forall2.
+    intros (?&?&?&E). rewrite E. econstructor; eauto.
+  * destruct (proj_bytes (rev_if_be vl2)) eqn:?.
+    { rewrite proj_pointer_undef, proj_pointer_seg_undef;
+        eauto using proj_bytes_not_inject, rev_if_be_forall2. }
+    destruct (proj_pointer (rev_if_be vl1)) as [[??]|] eqn:?.
+    { exploit (proj_pointer_inject f (rev_if_be vl1) (rev_if_be vl2));
+        eauto using rev_if_be_forall2.
+      intros (?&?&?&E). rewrite E. econstructor; eauto. }
+    destruct (proj_pointer_seg 4 (rev_if_be vl1)) as [[[??]?]|] eqn:?; [|constructor].
+    erewrite proj_pointer_seg_not_pointer by eauto using rev_if_be_forall2.
+    exploit (proj_pointer_seg_inject f (rev_if_be vl1) (rev_if_be vl2));
+      eauto using rev_if_be_forall2.
+    intros (?&?&?&E). rewrite E. econstructor; eauto.
 Qed.
 
 (** Symmetrically, [encode_val], applied to values related by [val_inject],
@@ -799,32 +1258,35 @@ Proof.
 Qed.
 
 Lemma repeat_Undef_inject_any:
-  forall f vl,
-  list_forall2 (memval_inject f) (list_repeat (length vl) Undef) vl.
+  forall f n vl,
+  n = length vl ->
+  list_forall2 (memval_inject f) (list_repeat n Undef) vl.
 Proof.
+  intros. subst.
   induction vl; simpl; constructor; auto. constructor. 
-Qed.  
+Qed.
 
 Lemma repeat_Undef_inject_self:
   forall f n,
   list_forall2 (memval_inject f) (list_repeat n Undef) (list_repeat n Undef).
 Proof.
   induction n; simpl; constructor; auto. constructor.
-Qed.  
+Qed.
 
 Theorem encode_val_inject:
   forall f v1 v2 chunk,
   val_inject f v1 v2 ->
   list_forall2 (memval_inject f) (encode_val chunk v1) (encode_val chunk v2).
 Proof.
-  intros. inv H; simpl.
-  destruct chunk; apply inj_bytes_inject || apply repeat_Undef_inject_self.
-  destruct chunk; apply inj_bytes_inject || apply repeat_Undef_inject_self.
-  destruct chunk; apply inj_bytes_inject || apply repeat_Undef_inject_self.
-  destruct chunk; try (apply repeat_Undef_inject_self). 
-  repeat econstructor; eauto. 
-  replace (size_chunk_nat chunk) with (length (encode_val chunk v2)).
-  apply repeat_Undef_inject_any. apply encode_val_length. 
+  intros. unfold encode_val. apply rev_if_be_forall2. inv H.
+  * destruct chunk; apply inj_bytes_inject || apply repeat_Undef_inject_self.
+  * destruct chunk; apply inj_bytes_inject || apply repeat_Undef_inject_self.
+  * destruct chunk; try (apply repeat_Undef_inject_self); repeat econstructor; eauto.
+  * destruct chunk; try (apply repeat_Undef_inject_self); repeat econstructor; eauto.
+  * destruct chunk; try (apply repeat_Undef_inject_self); repeat econstructor; eauto.
+  * apply repeat_Undef_inject_any.
+    now destruct v2, chunk; rewrite ?length_list_repeat,
+      ?length_inj_bytes, ?length_bytes_of_int.
 Qed.
 
 Definition memval_lessdef: memval -> memval -> Prop := memval_inject inject_id.
@@ -836,7 +1298,13 @@ Proof.
   unfold inject_id; reflexivity. rewrite Int.add_zero; auto. 
 Qed.
 
-(** [memval_inject] and compositions *)
+(** [memval_inject] and identity and compositions *)
+
+Lemma memval_inject_id:
+  forall v, memval_inject inject_id v v.
+Proof.
+  apply memval_lessdef_refl.
+Qed.
 
 Lemma memval_inject_compose:
   forall f f' v1 v2 v3,
@@ -844,150 +1312,10 @@ Lemma memval_inject_compose:
   memval_inject (compose_meminj f f') v1 v3.
 Proof.
   intros. inv H.
-  inv H0. constructor.
-  inv H0. econstructor. 
-  unfold compose_meminj; rewrite H1; rewrite H5; eauto. 
-  rewrite Int.add_assoc. decEq. unfold Int.add. apply Int.eqm_samerepr. auto with ints.
-  constructor.
+  * inv H0. constructor.
+  * inv H0. econstructor.
+    unfold compose_meminj; rewrite H1; rewrite H5; eauto.
+    rewrite Int.add_assoc. decEq. unfold Int.add. apply Int.eqm_samerepr. auto with ints.
+  * inv H0. constructor.
+  * constructor.
 Qed. 
-
-(** * Breaking 64-bit memory accesses into two 32-bit accesses *)
-
-Lemma int_of_bytes_append:
-  forall l2 l1, 
-  int_of_bytes (l1 ++ l2) = int_of_bytes l1 + int_of_bytes l2 * two_p (Z_of_nat (length l1) * 8).
-Proof.
-  induction l1; simpl int_of_bytes; intros.
-  simpl. ring.
-  simpl length. rewrite inj_S. 
-  replace (Z.succ (Z.of_nat (length l1)) * 8) with (Z_of_nat (length l1) * 8 + 8) by omega.
-  rewrite two_p_is_exp. change (two_p 8) with 256. rewrite IHl1. ring.
-  omega. omega.
-Qed.
-
-Lemma int_of_bytes_range:
-  forall l, 0 <= int_of_bytes l < two_p (Z_of_nat (length l) * 8).
-Proof.
-  induction l; intros. 
-  simpl. omega.
-  simpl length. rewrite inj_S. 
-  replace (Z.succ (Z.of_nat (length l)) * 8) with (Z.of_nat (length l) * 8 + 8) by omega.
-  rewrite two_p_is_exp. change (two_p 8) with 256. 
-  simpl int_of_bytes. generalize (Byte.unsigned_range a). 
-  change Byte.modulus with 256. omega. 
-  omega. omega. 
-Qed.
-
-Lemma length_proj_bytes:
-  forall l b, proj_bytes l = Some b -> length b = length l.
-Proof.
-  induction l; simpl; intros. 
-  inv H; auto.
-  destruct a; try discriminate. 
-  destruct (proj_bytes l) eqn:E; inv H. 
-  simpl. f_equal. auto.
-Qed.
-
-Lemma proj_bytes_append:
-  forall l2 l1,
-  proj_bytes (l1 ++ l2) =
-  match proj_bytes l1, proj_bytes l2 with
-  | Some b1, Some b2 => Some (b1 ++ b2)
-  | _, _ => None
-  end.
-Proof.
-  induction l1; simpl.
-  destruct (proj_bytes l2); auto.
-  destruct a; auto. rewrite IHl1. 
-  destruct (proj_bytes l1); auto. destruct (proj_bytes l2); auto. 
-Qed.
-
-Lemma decode_val_int64:
-  forall l1 l2,
-  length l1 = 4%nat -> length l2 = 4%nat ->
-  decode_val Mint64 (l1 ++ l2) =
-  Val.longofwords (decode_val Mint32 (if Archi.big_endian then l1 else l2))
-                  (decode_val Mint32 (if Archi.big_endian then l2 else l1)).
-Proof.
-  intros. unfold decode_val.
-  assert (PP: forall vl, match proj_pointer vl with Vundef => True | Vptr _ _ => True | _ => False end).
-    intros. unfold proj_pointer. destruct vl; auto. destruct m; auto. 
-    destruct (check_pointer 4 b i (Pointer b i n :: vl)); auto. 
-  assert (PP1: forall vl v2, Val.longofwords (proj_pointer vl) v2 = Vundef).
-    intros. generalize (PP vl). destruct (proj_pointer vl); reflexivity || contradiction.
-  assert (PP2: forall v1 vl, Val.longofwords v1 (proj_pointer vl) = Vundef).
-    intros. destruct v1; simpl; auto. 
-    generalize (PP vl). destruct (proj_pointer vl); reflexivity || contradiction.
-  rewrite proj_bytes_append. 
-  destruct (proj_bytes l1) as [b1|] eqn:B1; destruct (proj_bytes l2) as [b2|] eqn:B2.
-- exploit length_proj_bytes. eexact B1. rewrite H; intro L1.
-  exploit length_proj_bytes. eexact B2. rewrite H0; intro L2.
-  assert (UR: forall l, length l = 4%nat -> Int.unsigned (Int.repr (int_of_bytes l)) = int_of_bytes l).
-    intros. apply Int.unsigned_repr. 
-    generalize (int_of_bytes_range l). rewrite H1. 
-    change (two_p (Z.of_nat 4 * 8)) with (Int.max_unsigned + 1). 
-    omega.
-  unfold decode_int, rev_if_be. destruct Archi.big_endian; rewrite B1; rewrite B2.
-  + rewrite <- (rev_length b1) in L1. 
-    rewrite <- (rev_length b2) in L2.
-    rewrite rev_app_distr.
-    set (b1' := rev b1) in *; set (b2' := rev b2) in *.
-    unfold Val.longofwords. f_equal. rewrite Int64.ofwords_add. f_equal.
-    rewrite !UR by auto. rewrite int_of_bytes_append. 
-    rewrite L2. change (Z.of_nat 4 * 8) with 32. ring.
-  + unfold Val.longofwords. f_equal. rewrite Int64.ofwords_add. f_equal.
-    rewrite !UR by auto. rewrite int_of_bytes_append. 
-    rewrite L1. change (Z.of_nat 4 * 8) with 32. ring.
-- destruct Archi.big_endian; rewrite B1; rewrite B2; auto.
-- destruct Archi.big_endian; rewrite B1; rewrite B2; auto.
-- destruct Archi.big_endian; rewrite B1; rewrite B2; auto.
-Qed.
-
-Lemma bytes_of_int_append:
-  forall n2 x2 n1 x1,
-  0 <= x1 < two_p (Z_of_nat n1 * 8) ->
-  bytes_of_int (n1 + n2) (x1 + x2 * two_p (Z_of_nat n1 * 8)) =
-  bytes_of_int n1 x1 ++ bytes_of_int n2 x2.
-Proof.
-  induction n1; intros.
-- simpl in *. f_equal. omega. 
-- assert (E: two_p (Z.of_nat (S n1) * 8) = two_p (Z.of_nat n1 * 8) * 256).
-  {
-    rewrite inj_S. change 256 with (two_p 8). rewrite <- two_p_is_exp. 
-    f_equal. omega. omega. omega. 
-  }
-  rewrite E in *. simpl. f_equal.
-  apply Byte.eqm_samerepr. exists (x2 * two_p (Z.of_nat n1 * 8)). 
-  change Byte.modulus with 256. ring.
-  rewrite Zmult_assoc. rewrite Z_div_plus. apply IHn1.
-  apply Zdiv_interval_1. omega. apply two_p_gt_ZERO; omega. omega. 
-  assumption. omega.
-Qed.
-
-Lemma bytes_of_int64:
-  forall i,
-  bytes_of_int 8 (Int64.unsigned i) =
-  bytes_of_int 4 (Int.unsigned (Int64.loword i)) ++ bytes_of_int 4 (Int.unsigned (Int64.hiword i)).
-Proof.
-  intros. transitivity (bytes_of_int (4 + 4) (Int64.unsigned (Int64.ofwords (Int64.hiword i) (Int64.loword i)))).
-  f_equal. f_equal. rewrite Int64.ofwords_recompose. auto.
-  rewrite Int64.ofwords_add'.
-  change 32 with (Z_of_nat 4 * 8). 
-  rewrite Zplus_comm. apply bytes_of_int_append. apply Int.unsigned_range. 
-Qed.
-
-Lemma encode_val_int64:
-  forall v,
-  encode_val Mint64 v =
-     encode_val Mint32 (if Archi.big_endian then Val.hiword v else Val.loword v)
-  ++ encode_val Mint32 (if Archi.big_endian then Val.loword v else Val.hiword v).
-Proof.
-  intros. destruct v; destruct Archi.big_endian eqn:BI; try reflexivity;
-  unfold Val.loword, Val.hiword, encode_val.
-  unfold inj_bytes. rewrite <- map_app. f_equal. 
-  unfold encode_int, rev_if_be. rewrite BI. rewrite <- rev_app_distr. f_equal.
-  apply bytes_of_int64. 
-  unfold inj_bytes. rewrite <- map_app. f_equal. 
-  unfold encode_int, rev_if_be. rewrite BI.
-  apply bytes_of_int64.
-Qed.
