arm/Op.v
@@ -969,12 +969,12 @@ Lemma eval_condition_lessdef:
   eval_condition cond vl1 m1 = Some b ->
   eval_condition cond vl2 m2 = Some b.
 Proof.
-  intros. eapply eval_condition_inj with (f := fun b => Some(b, 0)) (m1 := m1).
+  intros. eapply eval_condition_inj with (f := inject_id) (m1 := m1).
   apply valid_pointer_extends; auto.
   apply weak_valid_pointer_extends; auto.
   apply weak_valid_pointer_no_overflow_extends.
   apply valid_different_pointers_extends; auto.
-  rewrite <- val_list_inject_lessdef. eauto. auto.
+  rewrite val_list_inject_id. eauto. auto.
 Qed.
 
 Lemma eval_operation_lessdef:
@@ -984,19 +984,19 @@ Lemma eval_operation_lessdef:
   eval_operation genv sp op vl1 m1 = Some v1 ->
   exists v2, eval_operation genv sp op vl2 m2 = Some v2 /\ Val.lessdef v1 v2.
 Proof.
-  intros. rewrite val_list_inject_lessdef in H.
+  intros. rewrite <-val_list_inject_id in H.
   assert (exists v2 : val,
           eval_operation genv sp op vl2 m2 = Some v2
-          /\ val_inject (fun b => Some(b, 0)) v1 v2).
+          /\ val_inject inject_id v1 v2).
   eapply eval_operation_inj with (m1 := m1) (sp1 := sp).
-  intros. rewrite <- val_inject_lessdef; auto.
+  intros. rewrite val_inject_id; auto.
   apply valid_pointer_extends; auto.
   apply weak_valid_pointer_extends; auto.
   apply weak_valid_pointer_no_overflow_extends.
   apply valid_different_pointers_extends; auto.
-  rewrite <- val_inject_lessdef; auto.
+  rewrite val_inject_id; auto.
   eauto. auto. 
-  destruct H2 as [v2 [A B]]. exists v2; split; auto. rewrite val_inject_lessdef; auto. 
+  destruct H2 as [v2 [A B]]. exists v2; split; auto. apply val_inject_id; auto. 
 Qed.
 
 Lemma eval_addressing_lessdef:
@@ -1005,15 +1005,15 @@ Lemma eval_addressing_lessdef:
   eval_addressing genv sp addr vl1 = Some v1 ->
   exists v2, eval_addressing genv sp addr vl2 = Some v2 /\ Val.lessdef v1 v2.
 Proof.
-  intros. rewrite val_list_inject_lessdef in H.
+  intros. rewrite <-val_list_inject_id in H.
   assert (exists v2 : val,
           eval_addressing genv sp addr vl2 = Some v2
-          /\ val_inject (fun b => Some(b, 0)) v1 v2).
+          /\ val_inject inject_id v1 v2).
   eapply eval_addressing_inj with (sp1 := sp).
-  intros. rewrite <- val_inject_lessdef; auto. 
-  rewrite <- val_inject_lessdef; auto. 
+  intros. rewrite val_inject_id; auto. 
+  rewrite val_inject_id; auto. 
   eauto. auto. 
-  destruct H1 as [v2 [A B]]. exists v2; split; auto. rewrite val_inject_lessdef; auto. 
+  destruct H1 as [v2 [A B]]. exists v2; split; auto. apply val_inject_id; auto. 
 Qed.
 
 End EVAL_LESSDEF.
@@ -1087,4 +1087,3 @@ Proof.
 Qed.
 
 End EVAL_INJECT.
-
